proved one implication for interp preserving bind, interp ret

src/coq/Utils/InterpProp.v
@@ -35,7 +35,6 @@ Require Import Paco.paco.
 Import ListNotations.
 Import ITree.Basics.Basics.Monads.
 
-
 Import MonadNotation.
 Import CatNotations.
 Local Open Scope monad_scope.
@@ -70,19 +69,35 @@ Section interp_prop.
              (k_spec : forall T R, E T -> itree F T -> (T -> itree E R) -> (T -> itree F R) -> itree F R -> Prop) : Prop
     := forall T R e k1 k2 t2, t2 ≈ bind (h T e) k2 -> k_spec T R e (h T e) k1 k2 t2.
 
-  Inductive interp_PropTF {E F}
-            (h_spec : E ~> PropT F)
-            (k_spec : forall T R, E T -> itree F T -> (T -> itree E R) -> (T -> itree F R) -> itree F R -> Prop)
+  Context {E F : Type -> Type}.
+  Context (h_spec : E ~> PropT F).
+  Context (k_spec : forall T R, E T -> itree F T -> (T -> itree F R) -> itree F R -> Prop).
+
+  (* Well-formedness conditions for k_specs *)
+  Class k_spec_WF := {
+      k_spec_Returns: forall {A R} ta k2 t2 e,
+        k_spec A R e ta k2 t2 -> forall a, Returns a ta -> forall a', Returns a' (k2 a) -> Returns a' t2;
+      k_spec_bind: forall {A R} ta k2 (t2 : itree F R) e (k' : _ -> itree F R),
+        k_spec A R e ta k2 t2 ->
+        k_spec A R e ta (fun x => bind (k2 x) k') (bind t2 k')
+    }.
+
+  Context (k_spec_wellformed : k_spec_WF).
+
+  Inductive interp_PropTF
             {R : Type} (RR : relation R) (sim : itree E R -> itree F R -> Prop)
-            : itree' E R -> itree F R -> Prop :=
+            : itree' E R -> itree' F R -> Prop :=
   | Interp_PropT_Ret : forall r1 r2 (REL: RR r1 r2),
-      interp_PropTF h_spec k_spec RR sim (RetF r1) (Ret r2)
+      interp_PropTF RR sim (RetF r1) (RetF r2)
 
   | Interp_PropT_Tau : forall t1 t2 (HS: sim t1 t2),
-      interp_PropTF h_spec k_spec RR sim (TauF t1) (Tau t2)
+      interp_PropTF RR sim (TauF t1) (TauF t2)
 
-  | Interp_PropT_TauP : forall t1 t2 (HS: interp_PropTF h_spec k_spec RR sim (observe t1) t2),
-      interp_PropTF h_spec k_spec RR sim (TauF t1) t2
+  | Interp_PropT_TauL : forall t1 t2 (HS: interp_PropTF RR sim (observe t1) t2),
+      interp_PropTF RR sim (TauF t1) t2
+
+  | Interp_PropT_TauR : forall t1 t2 (HS: interp_PropTF RR sim t1 (observe t2)),
+      interp_PropTF RR sim t1 (TauF t2)
 
   | Interp_PropT_Vis : forall A (e : E A) (k1 : A -> itree E R)
                          (t2 : itree F R)
@@ -95,327 +110,252 @@ Section interp_prop.
 
                          (* k_spec => t2 ≈ bind ta k2 *)
                          (* k_spec => True *)
-                         (KS : k_spec A R e ta k1 k2 t2), 
-      interp_PropTF h_spec k_spec RR sim (VisF e k1) t2.
+                         (KS : k_spec A R e ta k2 t2),
+      interp_PropTF RR sim (VisF e k1) (observe t2).
 
   Hint Constructors interp_PropTF : core.
 
-  Lemma interp_PropTF_mono E F h_spec k_spec R RR  (t0 : itree' E R) (t1 : itree F R) sim sim'
-        (IN : interp_PropTF h_spec k_spec RR sim t0 t1)
-        (LE : sim <2= sim') : 
-    (interp_PropTF h_spec k_spec RR sim' t0 t1).
+  Lemma interp_PropTF_mono R RR (t0 : itree' E R) (t1 : itree' F R) sim sim'
+        (IN : interp_PropTF RR sim t0 t1)
+        (LE : sim <2= sim') :
+    (interp_PropTF RR sim' t0 t1).
   Proof.
     induction IN; eauto.
   Qed.
 
   Hint Resolve interp_PropTF_mono : paco.
 
-  Definition interp_PropT_ E F h_spec k_spec R RR sim (t0 : itree E R) (t1 : itree F R) :=
-    interp_PropTF h_spec k_spec RR sim (observe t0) t1.
+  Definition interp_PropT_ R RR sim (t0 : itree E R) (t1 : itree F R) :=
+    interp_PropTF RR sim (observe t0) (observe t1).
   Hint Unfold interp_PropT_ : core.
 
-  Lemma interp_PropT__mono E F h_spec k_spec R RR : monotone2 (interp_PropT_ E F h_spec k_spec R RR).
+  Lemma interp_PropT__mono R RR : monotone2 (interp_PropT_ R RR).
   Proof.
     do 2 red. intros. eapply interp_PropTF_mono; eauto.
   Qed.
   Hint Resolve interp_PropT__mono : paco.
 
   (* Definition 5.2 *)
-  Definition interp_prop {E F}
-            (h_spec : E ~> PropT F)
-            (k_spec : forall T R, E T -> itree F T -> (T -> itree E R) -> (T -> itree F R) -> itree F R -> Prop)
-    :
+  Definition interp_prop :
     forall R (RR: relation R), itree E R -> PropT F R :=
-      fun R (RR: relation R) =>  paco2 (interp_PropT_ E F h_spec k_spec R RR) bot2.
+      fun R (RR: relation R) =>  paco2 (interp_PropT_ R RR) bot2.
 
-  (* #[global] Instance interp_PropTF_Proper *)
-  (*  {E F} *)
-  (*  (h_spec : E ~> PropT F) *)
-  (*  (k_spec : forall T R, E T -> itree F T -> (T -> itree E R) -> (T -> itree F R) -> itree F R -> Prop) *)
-  (*  R RR (t : itree' E R) *)
-  (*        (sim : itree E R -> itree F R -> Prop) *)
-  (*        (HS: forall t, Proper(eutt eq ==> flip impl) (sim t)) *)
-  (*        (KS: forall A R e ta k1 k2, Proper (eutt eq ==> flip impl) (k_spec A R e ta k1 k2)) *)
-  (*   :  *)
-  (*   Proper(eutt eq ==> iff) (interp_PropTF h_spec k_spec RR sim t). *)
-  (* Proof. *)
-  (*   do 2 red. *)
-  (*   intros. *)
-  (*   split; intros. *)
-  (*   - inversion H0; subst; econstructor; eauto. *)
-  (*     + rewrite <- H. assumption. *)
-  (*     + specialize (HS t1). rewrite <- H. assumption. *)
-  (*     + (* h_spec now depends on the tree `t2`, so we need to show that it respects x ≈ y *) *)
-  (*       (* Not a guarantee, depends on what h_spec is... So we need a proper instance for that *) *)
-  (*       rewrite <- H; auto. *)
-  (*   - inversion H0; subst; econstructor; eauto. *)
-  (*     rewrite H. assumption. specialize (HS t1). rewrite H. assumption. *)
-  (*     rewrite H. assumption. *)
-  (* Qed. *)
+  Arguments interp_prop {_}.
+
+  Instance interp_prop_Proper_impl :
+    forall R (x : _ R), Proper (eutt eq ==> impl) (interp_prop eq x).
+  Proof.
+    repeat intro. red in H0.
+    punfold H; punfold H0; red in H; red in H0; cbn in *.
+    remember (observe x); remember (observe x0); remember (observe y).
+    revert_until H. clear Heqi0 x0. revert x.
+    pcofix CIH.
+    intros; induction H; subst.
+    - eapply paco2_mon. pstep; red; try rewrite <- Heqi1; eauto.
+      intros; inv PR.
+    - pstep; red; rewrite <- Heqi1. inv H1; pclearbot.
+      + constructor. right.
+  Abort.
+
+  Instance interp_prop_eq_itree_Proper :
+    forall R, Proper (eq_itree eq ==> eq_itree eq ==> iff) (interp_prop (R := R) eq).
+  Proof.
+    repeat intro.
+  Admitted.
+
+  Instance interp_prop_eutt_Proper :
+    forall R x, Proper (eutt eq ==> iff) (interp_prop (R := R) eq x).
+  Proof.
+    repeat intro.
+  Admitted.
+
   (* Figure 7: Interpreter law for Ret *)
   Lemma interp_prop_ret :
-    forall R E F
-      (h_spec : E ~> PropT F)
-      (k_spec : forall T R, E T -> itree F T -> (T -> itree E R) -> (T -> itree F R) -> itree F R -> Prop)
-      (r : R)
-    , Eq1_PropT _ (interp_prop h_spec k_spec R eq (ret r)) (ret r).
+    forall R (r : R),
+      (interp_prop eq (ret r) ≈ ret r)%monad.
   Proof.
     intros.
     repeat red.
     split; [| split].
     - intros. split; intros.
-      + unfold interp_prop in H0.
-        pinversion H0. subst.
-        cbn. rewrite <- H. reflexivity.
-      + pstep. red. do 2 red in H0.
-        rewrite H0 in H.
-
-   (*      rewrite H. eapply Interp_PropT_Ret. cbn. econstructor. reflexivity. rewrite H. cbn in H0. assumption. *)
-   (*  - do 3 red. *)
-   (*    intros t1 t2 eq; split; intros H; pinversion H; subst. *)
-   (*    + red. pstep. econstructor. reflexivity. rewrite <- eq. assumption. *)
-   (*    + red. pstep. econstructor. reflexivity. rewrite eq. assumption. *)
-   (* - do 3 red. intros. split; intros; cbn in *. rewrite <- H. assumption. rewrite H; assumption. *)
-  Admitted.
-
-  #[global] Instance interp_prop_Proper
-   {E F}
-   (h_spec : E ~> PropT F)
-   (k_spec : forall T R, E T -> itree F T -> (T -> itree E R) -> (T -> itree F R) -> itree F R -> Prop)
-   R RR (t : itree E R)
-   (KS: forall A R e ta k1 k2, Proper (eutt eq ==> flip impl) (k_spec A R e ta k1 k2)) :
-    Proper(eq_itree Logic.eq ==> iff) (interp_prop h_spec k_spec R RR t).
-  Proof.
-    do 2 red.
-    intros.
-    split.
-    - revert t x y H.
-      pcofix CIH.
-      intros t x y eq HI.
-      red in HI. punfold HI. red in HI.
-      pstep. red. genobs t ot.
-    (*   inversion HI; subst; econstructor; eauto. *)
-    (*   + rewrite <- eq. assumption. *)
-    (*   + pclearbot. right. eapply CIH; eauto. *)
-    (*   + intros. specialize (HK a H0). pclearbot. right. eapply CIH. 2 : { apply HK. } reflexivity. *)
-    (*   + rewrite <- eq. eauto. *)
-    (* - revert t x y H. *)
-    (*   pcofix CIH. *)
-    (*   intros t x y eq HI. *)
-    (*   red in HI. punfold HI. red in HI. *)
-    (*   pstep. red. genobs t ot. *)
-    (*   inversion HI; subst; econstructor; eauto. *)
-    (*   + rewrite eq. assumption. *)
-    (*   + pclearbot. right. eapply CIH; eauto. *)
-    (*   + intros. specialize (HK a H0). pclearbot. right. eapply CIH. 2 : { apply HK. } reflexivity. *)
-      (*   + rewrite eq. eauto. *)
-  Admitted.
-
-  #[global] Instance interp_prop_Proper2
-   {E F}
-   (h_spec : E ~> PropT F)
-   (k_spec : forall T R, E T -> itree F T -> (T -> itree E R) -> (T -> itree F R) -> itree F R -> Prop)
-   R RR (t : itree E R)
-   (KS: forall A R e ta k1 k2, Proper (eutt eq ==> flip impl) (k_spec A R e ta k1 k2)) :
-    Proper(eutt Logic.eq ==> iff) (interp_prop h_spec k_spec R RR t).
-  Proof.
-    do 2 red.
-    intros.
-    split.
-    - revert t x y H.
-      pcofix CIH.
-      intros t x y eq HI.
-      red in HI. punfold HI. red in HI.
-      pstep. red. genobs t ot.
-    (*   inversion HI; subst; econstructor; eauto. *)
-    (*   + rewrite <- eq. assumption. *)
-    (*   + pclearbot. right. eapply CIH; eauto. *)
-    (*   + intros. specialize (HK a H0). pclearbot. right. eapply CIH. 2 : { apply HK. } reflexivity. *)
-    (*   + rewrite <- eq. eauto. *)
-    (* - revert t x y H. *)
-    (*   pcofix CIH. *)
-    (*   intros t x y eq HI. *)
-    (*   red in HI. punfold HI. red in HI. *)
-    (*   pstep. red. genobs t ot. *)
-    (*   inversion HI; subst; econstructor; eauto. *)
-    (*   + rewrite eq. assumption. *)
-    (*   + pclearbot. right. eapply CIH; eauto. *)
-    (*   + intros. specialize (HK a H0). pclearbot. right. eapply CIH. 2 : { apply HK. } reflexivity. *)
-      (*   + rewrite eq. eauto. *)
-  Admitted.
-
-  (* TODO: Move this *)
-  Lemma eqit_flip_symmetric {E R} (RR : R -> R -> Prop) `{Symmetric R RR} b1 b2:
-    forall (u : itree E R) (v : itree E R),
-      eqit RR b1 b2 u v -> eqit (flip RR) b1 b2 u v.
-  Proof.
-    pcofix self; pstep. intros u v euv. punfold euv.
-    red in euv |- *. induction euv; pclearbot; eauto 7 with paco.
+      + punfold H0. red in H0; cbn in H0.
+        punfold H; red in H.
+        remember (RetF r); remember (observe x).
+        revert x Heqi0 H Heqi.
+        induction H0; intros; try inv Heqi; subst; auto.
+        * intros; subst; cbn.
+          symmetry; pstep; auto.
+        * eapply IHinterp_PropTF; eauto.
+          assert (Tau t2 ≈ y) by (pstep; auto). rewrite tau_eutt in H1.
+          punfold H1; auto.
+      + do 2 red in H0. rewrite <- H in H0. clear H.
+        punfold H0; red in H0; cbn in H0.
+        pstep; red; cbn.
+        remember (observe x); remember (RetF r).
+        revert x r Heqi Heqi0. clear y.
+        induction H0; intros; try inv Heqi0; subst; auto.
+        constructor; eapply IHeqitF; eauto.
+    - do 3 red. intros; split; intros; [rewrite <- H | rewrite H] ; auto.
+    - do 3 red. intros. split; intros; cbn in *. rewrite <- H. assumption. rewrite H; assumption.
   Qed.
 
-  #[global] Instance interp_prop_Proper3
-   {E F} {a b}
-   (h_spec : E ~> PropT F)
-   (k_spec : forall T R, E T -> itree F T -> (T -> itree E R) -> (T -> itree F R) -> itree F R -> Prop)
-   (KP : forall T R RR b a, Proper (eq ==> eq ==> (fun k1 k2 => forall x, eqit RR b a (k1 x) (k2 x)) ==> eq ==> eq ==> iff) (k_spec T R))
-   R RR :
-    Proper(eqit eq a b ==> eq  ==> iff) (interp_prop h_spec k_spec R RR).
+  From ITree Require Import Eq.EqAxiom.
+
+  (* Interp bind law *)
+  Lemma interp_prop_bind :
+    forall R (t : _ R) (k : R -> _ R),
+      (interp_prop eq (bind t k) ≈
+                   bind (interp_prop eq t) (fun x => interp_prop eq (k x)))%monad.
   Proof.
-    do 4 red.
-    intros; split.
-    - subst.
-      revert x y H y0.
-      pcofix CIH.
-      intros x y eq t H.
-      pstep; red.
-      punfold H. red in H.
+    intros R t k.
+    repeat red.
+    split; [| split]; cycle 1.
+    { do 3 red. intros; split; intros; [rewrite <- H | rewrite H] ; auto. }
+    { do 3 red. intros. split; intros; cbn in *. rewrite <- H. assumption. rewrite H; assumption. }
+    split; intros; cycle 1; [ rewrite H | rewrite <- H]; clear H.
+    - destruct H0 as (?&?&?&?&?).
+      rewrite H0. clear H0. clear y.
+      setoid_rewrite unfold_bind.
+      match goal with
+      | |- interp_prop _ ?l ?r => remember l; remember r
+      end.
+      revert_until R. pcofix CIH. intros.
+      punfold H0; red in H0; cbn in H0.
+      clear x. rename t into x, x2 into x'.
+      rename x3 into k', i0 into i'.
 
-      punfold eq. red in eq.
-      genobs x obsx.
-      genobs y obsy.
-      revert x y Heqobsx Heqobsy t H.
+      remember (observe x); remember (observe x').
+      revert_until H0. revert x x' Heqi1 Heqi2.
+      induction H0; intros.
+      + subst; eauto. setoid_rewrite (itree_eta x') in H1.
+        rewrite <- Heqi2 in H1.
+        assert (Returns (E := F) r2 (Ret r2)) by (econstructor; reflexivity).
+        specialize (H1 _ H). eapply paco2_mon. punfold H1.
+        intros; inv PR.
+      + (* coinductive tau *)
+        pstep. subst. constructor. right. eapply CIH.
+        4,5:eapply bisimulation_is_eq; rewrite unfold_bind; reflexivity.
+        { auto. }
+        pclearbot. punfold HS. pstep. eapply HS.
+        intros; eapply H1. rewrite (itree_eta x').
+        rewrite <- Heqi2. eapply ReturnsTau; eauto. reflexivity.
+      + rewrite Heqi. pstep. constructor.
+        specialize (IHinterp_PropTF t1 x' eq_refl Heqi2 H1 (bind t1 k)).
 
-      induction eq; intros x y Heqobsx Heqobsy t H; inversion H; subst; pclearbot.
-      + econstructor; eauto.
-      + econstructor. right. eapply CIH. apply REL. apply HS.
-   (*    + apply inj_pair2 in H2. *)
-   (*      apply inj_pair2 in H3. subst. *)
-   (*      econstructor; eauto. intros X HX. specialize (REL X). specialize (HK X HX). pclearbot. *)
-   (*      right. *)
+        assert (H' : x <- t1;; k x =
+                    match observe t1 with
+                    | RetF r => k r
+                    | TauF t => Tau (ITree.bind t k)
+                    | @VisF _ _ _ X e ke => Vis e (fun x : X => ITree.bind (ke x) k)
+                    end).
+        {
+          apply bisimulation_is_eq; setoid_rewrite unfold_bind; reflexivity.
+        }
+        specialize (IHinterp_PropTF H' _ Heqi0).
+        punfold IHinterp_PropTF.
+      + rewrite Heqi0. pstep. constructor.
+        specialize (IHinterp_PropTF _ t2 Heqi1 eq_refl).
+        assert (forall a : R, Returns a t2 -> interp_prop eq (k a) (k' a)).
+        { intros; eapply H1. rewrite (itree_eta x'); rewrite <- Heqi2.
+          rewrite tau_eutt; auto. }
+        specialize (IHinterp_PropTF H _ Heqi (bind t2 k')).
 
-   (*      eapply CIH; eauto. *)
-   (*      eapply KP; eauto. *)
-   (*      intros. *)
-   (*      eapply eqit_flip; *)
-   (*      eapply eqit_flip_symmetric; eauto; typeclasses eauto. *)
-   (*    + eapply IHeq.  reflexivity. reflexivity. *)
-   (*      punfold HS. *)
-   (*    + econstructor. left. pstep. eapply IHeq. reflexivity. reflexivity. assumption. *)
-   (*    + econstructor. left.  pstep. eapply IHeq. reflexivity. reflexivity. assumption. *)
-   (*    + econstructor. left.  pstep. eapply IHeq. reflexivity. reflexivity. assumption. *)
+        assert (H' : x <- t2;; k' x =
+                    match observe t2 with
+                    | RetF r => k' r
+                    | TauF t => Tau (ITree.bind t k')
+                    | @VisF _ _ _ X e ke => Vis e (fun x : X => ITree.bind (ke x) k')
+                    end).
+        {
+          apply bisimulation_is_eq; setoid_rewrite unfold_bind; reflexivity.
+        }
+        specialize (IHinterp_PropTF H').
+        punfold IHinterp_PropTF.
+      + rewrite Heqi. pstep. econstructor; [ eauto | ..].
+        * intros. specialize (HK _ H). pclearbot.
+          right. eapply CIH; [ auto | ..].
+          3,4 :eapply bisimulation_is_eq; setoid_rewrite <- unfold_bind; reflexivity.
+          eauto.
+          intros; eapply H1. rewrite (itree_eta x'). rewrite <- Heqi2.
+          rewrite <- itree_eta.
+          eapply k_spec_Returns; eauto.
+        * match goal with
+          | |- k_spec _ _ _ _ ?l _ => remember l
+          end.
+          assert (i0 = (fun a => k2 a >>= k')). {
+            apply FunctionalExtensionality.functional_extensionality.
+            intros; apply bisimulation_is_eq. rewrite Heqi3.
+            rewrite <- unfold_bind; reflexivity.
+          }
+          assert (i' = t2 >>= k'). {
+            apply bisimulation_is_eq. rewrite Heqi0; rewrite <- unfold_bind; reflexivity.
+          }
+          rewrite H, H0. eapply k_spec_bind; eauto.
+    - (* tricky case : need to use classical reasoning to
+       case-analyze on whether prefix of tree is finite *)
+      (* punfold H0. red in H0; cbn in H0. *)
+      (* punfold H; red in H. *)
+      (* repeat red. repeat red in spec. *)
+      (* remember (observe *)
+      (*       match observe t with *)
+      (*       | RetF r => k r *)
+      (*       | TauF t => Tau (ITree.bind t k) *)
+      (*       | @VisF _ _ _ X e ke => Vis e (fun x : X => ITree.bind (ke x) k) *)
+      (*       end) ; remember (observe x). remember (observe y). *)
+      (* revert x Heqi0 H Heqi. *)
+      (* induction H0; intros; try inv Heqi; subst; auto. *)
+      (* + intros; subst; cbn. *)
+      (*   destruct (observe t) eqn: Ht; try inv H1. *)
+      (*   eexists (ret r), (fun x => ret r2). *)
+      (*   split; [ | split]; eauto. *)
+      (*   * pstep; red; rewrite Ht; constructor; auto. *)
+      (*   * setoid_rewrite Eq.bind_ret_l. symmetry; pstep; auto. *)
+      (*   * intros. eapply Returns_ret_inv in H0; subst. *)
+      (*     pstep; red; rewrite <- H2; constructor; auto. *)
+      (* + destruct (observe t) eqn: Ht; try inv H1. *)
+      (*   * eexists (ret r), (fun _ => _). *)
+      (*     split; [ pstep; red; rewrite Ht; constructor; auto | ]. *)
+      (*     split; [ rewrite bind_ret_l; reflexivity | ]. *)
+      (*     intros. eapply Returns_ret_inv in H0; subst. *)
+      (*     pclearbot. *)
+      (*     pcofix CIH. *)
 
-   (* - subst. *)
-   (*    revert x y H y0. *)
-   (*    pcofix CIH. *)
-   (*    intros x y eq t H. *)
-   (*    pstep; red. *)
-   (*    punfold H. red in H. *)
-
-   (*    punfold eq. red in eq. *)
-   (*    genobs x obsx. *)
-   (*    genobs y obsy. *)
-   (*    revert x y Heqobsx Heqobsy t H. *)
-
-   (*    induction eq; intros x y Heqobsx Heqobsy t H; inversion H; subst; pclearbot. *)
-   (*    + econstructor; eauto. *)
-   (*    + econstructor. right. eapply CIH. apply REL. apply HS. *)
-   (*    + apply inj_pair2 in H2. *)
-   (*      apply inj_pair2 in H3. subst. *)
-   (*      econstructor; eauto. intros X HX. specialize (REL X). specialize (HK X HX). pclearbot. *)
-   (*      right. *)
-
-   (*      eapply CIH; eauto. *)
-   (*      eapply KP; eauto. *)
-   (*    + econstructor. left. pstep. eapply IHeq. reflexivity. reflexivity. assumption. *)
-   (*    + econstructor. left. pstep. eapply IHeq. reflexivity. reflexivity. assumption. *)
-   (*    + econstructor. left. pstep. eapply IHeq. reflexivity. reflexivity. assumption. *)
-        (*    + eapply IHeq. reflexivity. reflexivity.   punfold HS. *)
+          (* pstep; red; rewrite <- H2. constructor; auto. *)
+      admit.
   Admitted.
 
-    Lemma interp_prop_ret_pure :
-      forall {T E F} (RR : relation T) `{REF: Reflexive _ RR} (x : T)
-        (h : E ~> PropT F)
-        (k_spec : forall T R, E T -> itree F T -> (T -> itree E R) -> (T -> itree F R) -> itree F R -> Prop),
-      interp_prop h k_spec _ RR (ret x) (ret x).
-    Proof.
-      intros T E F RR REF x h k_spec.
-      generalize dependent x.
-      pcofix CIH.
-      intros x.
-      pstep.
-      cbn.
-      econstructor.
-      reflexivity.
-    Qed.
- 
-    Lemma interp_prop_ret_refine :
-      forall {T E F} (RR : relation T) (x y : T)
-        (h : E ~> PropT F)
-        (k_spec : forall T R, E T -> itree F T -> (T -> itree E R) -> (T -> itree F R) -> itree F R -> Prop),
-        RR x y ->
-        interp_prop h k_spec _ RR (ret x) (ret y).
-    Proof.
-      intros T E F RR x y h k_spec RRxy.
-      generalize dependent y.
-      generalize dependent x.
-      pcofix CIH.
-      intros x y RRxy.
-      pstep.
-      cbn.
-      econstructor; eauto.
-    Qed.
+  Lemma interp_prop_ret_pure :
+    forall {T E F} (RR : relation T) `{REF: Reflexive _ RR} (x : T)
+      (h : E ~> PropT F)
+      (k_spec : forall T R, E T -> itree F T -> (T -> itree E R) -> (T -> itree F R) -> itree F R -> Prop),
+    interp_prop h k_spec _ RR (ret x) (ret x).
+  Proof.
+    intros T E F RR REF x h k_spec.
+    generalize dependent x.
+    pcofix CIH.
+    intros x.
+    pstep.
+    cbn.
+    econstructor.
+    reflexivity.
+  Qed.
 
-    Lemma interp_prop_refl_h :
-      forall {T E} (RR : relation T) `{REF: Reflexive _ RR} (t1 t2 : itree E T)
-        (h : E ~> PropT E)
-        (k_spec : forall T R, E T -> itree E T -> (T -> itree E R) -> (T -> itree E R) -> itree E R -> Prop),
-        (forall {X : Type} (e : E X), h X e (trigger e)) ->
-        (k_spec_correct (fun T e => trigger e) k_spec) ->
-        t1 ≈ t2 ->
-        interp_prop h k_spec _ RR t1 t2.
-    Proof.
-      intros T E RR REF t1 t2 h k_spec H_SPEC K_SPEC EQ.
-      generalize dependent t2.
-      generalize dependent t1.
-      pcofix CIH.
-      intros t1 t2 EQ.
-      pose proof (itree_eta t1) as ETA.
-      destruct (observe t1) eqn:Ht1.
-      - pstep.
-        red.
-        rewrite Ht1.
-      (*   econstructor. *)
-      (*   reflexivity. *)
-      (*   rewrite <- EQ. *)
-      (*   rewrite ETA. *)
-      (*   reflexivity. *)
-      (* - pstep. *)
-      (*   red. *)
-      (*   rewrite Ht1. *)
-      (*   econstructor. *)
-      (*   right. *)
-      (*   apply CIH; auto. *)
-      (*   rewrite <- tau_eutt. *)
-      (*   rewrite <- ETA. *)
-      (*   auto. *)
-      (* - pstep. *)
-      (*   red. *)
-      (*   rewrite Ht1. *)
-      (*   eapply Interp_PropT_Vis with (k2 := k). *)
-      (*   + eauto. *)
-      (*   + intros a RET. *)
-      (*     right. *)
-      (*     apply CIH. *)
-      (*     reflexivity. *)
-      (*   + eapply K_SPEC. rewrite <- EQ. *)
-      (*     setoid_rewrite bind_trigger. *)
-      (*     cbn. *)
-      (*     rewrite ETA. *)
-        (*     reflexivity. *)
-    Admitted.
-
-    Lemma interp_prop_refl :
-      forall {T E} (RR : relation T) `{REF: Reflexive _ RR} (t : itree E T)
-        (h : forall X : Type, E X -> PropT E X)
-        (k_spec : forall T R, E T -> itree E T -> (T -> itree E R) -> (T -> itree E R) -> itree E R -> Prop),
-        (forall {X : Type} (e : E X), h X e (trigger e)) ->
-        (k_spec_correct (fun T e => trigger e) k_spec) ->
-        interp_prop h k_spec _ RR t t.
-    Proof.
-      intros T E RR REF t h k_spec H_SPEC K_SPEC.
-      apply interp_prop_refl_h; eauto.
-      reflexivity.
-    Qed.
+  Lemma interp_prop_ret_refine :
+    forall {T E F} (RR : relation T) (x y : T)
+      (h : E ~> PropT F)
+      (k_spec : forall T R, E T -> itree F T -> (T -> itree E R) -> (T -> itree F R) -> itree F R -> Prop),
+      RR x y ->
+      interp_prop h k_spec _ RR (ret x) (ret y).
+  Proof.
+    intros T E F RR x y h k_spec RRxy.
+    generalize dependent y.
+    generalize dependent x.
+    pcofix CIH.
+    intros x y RRxy.
+    pstep.
+    cbn.
+    econstructor; eauto.
+  Qed.
 
   (* Lemma 5.4: interp_prop_correct - note that the paper presents a slightly simpler formulation where t = t' *)
   Lemma interp_prop_correct_exec:
@@ -449,7 +389,7 @@ Section interp_prop.
     (*   reflexivity. *)
 
     (*   unfold k_spec_correct in KC. *)
-      
+
     (*   eapply KC. *)
     (*   rewrite <- eq. *)
     (*   rewrite unfold_iter. *)
@@ -463,84 +403,6 @@ Section interp_prop.
     (*   rewrite tau_eutt. *)
     (*   reflexivity. *)
   Admitted.
-
-  (* Lemma 5.5 - note that the paper presents this lemma after unfolding the definition of Proper.
-   *)
-  Instance interp_prop_Proper_eq :
-    forall R (RR : relation R) (HR: Reflexive RR) (HT : Transitive RR) E F
-      (h_spec : E ~> PropT F)
-      (k_spec : forall T R, E T -> itree F T -> (T -> itree E R) -> (T -> itree F R) -> itree F R -> Prop)
-      (KP : forall T R RR b a, Proper (eq ==> eq ==> (fun k1 k2 => forall x, eqit RR b a (k1 x) (k2 x)) ==> eq ==> eq ==> iff) (k_spec T R)),
-      Proper (@eutt _ _ _ RR ==> eq ==> flip Basics.impl) (@interp_prop E _ h_spec k_spec R RR).
-  Proof.
-    intros.
-
-    do 5 red.
-    intros t1 t2 eqt s' s eqs HI.
-    subst.
-
-    revert t1 t2 eqt s HI.
-
-    pcofix CIH.
-
-    intros.
-
-    pstep. red.
-    punfold HI. red in HI.
-
-    punfold eqt. red in eqt.
-    genobs t1 obst1.
-    genobs t2 obst2.
-    revert t1 t2 Heqobst1 Heqobst2 s HI.
-
-    induction eqt; intros.
-    - inversion HI; subst.
-      econstructor. etransitivity; eauto.
-    (*   assumption. *)
-    (* - inversion HI; subst. *)
-    (*   econstructor. pclearbot. right.  eapply CIH; eauto. *)
-    (* - inversion HI. *)
-    (*   subst. *)
-    (*   apply inj_pair2 in H1. *)
-    (*   apply inj_pair2 in H2. *)
-    (*   subst. *)
-    (*   econstructor. *)
-    (*   apply HTA. *)
-    (*   intros a Ha. specialize (REL a). specialize (HK a Ha). red in REL. pclearbot. *)
-    (*   right. eapply CIH. apply REL. apply HK. *)
-    (*   eapply KP; eauto. *)
-    (*   pclearbot. *)
-    (*   intros x. *)
-    (*   eapply REL. *)
-    (* - econstructor. *)
-    (*   left. pstep. red. eapply IHeqt. reflexivity. eassumption. assumption. *)
-    (* - inversion HI; subst. *)
-    (*   pclearbot. *)
-    (*   eapply IHeqt. reflexivity. reflexivity. *)
-    (*   pinversion HS. *)
-      Admitted.
-  (* Qed. *)
-
-    Lemma interp_prop_trans :
-      forall {T E} (RR : relation T) `{REF: Reflexive _ RR} `{TRANS: Transitive _ RR} (x y z : itree E T)
-        (h : forall X : Type, E X -> PropT E X)
-        (k_spec : forall T R, E T -> itree E T -> (T -> itree E R) -> (T -> itree E R) -> itree E R -> Prop),
-        (forall {X : Type} (e : E X), h X e (trigger e)) ->
-        (k_spec_correct (fun T e => trigger e) k_spec) ->
-        interp_prop h k_spec _ RR x y ->
-        interp_prop h k_spec _ RR y z ->
-        interp_prop h k_spec _ RR x z.
-    Proof.
-      intros T E RR REF TRANS x y z h k_spec H_SPEC K_SPEC XY YZ.
-      revert x y z XY YZ.
-      pcofix CIH; intros x y z XY YZ.
-
-      punfold XY; punfold YZ; pfold; red in XY, YZ |- *.
-      genobs x xo.
-      genobs y yo.
-      genobs z zo.
-    Abort.
-
 
   (* Figure 7: interp Trigger law *)
   (* morally, we should only work with "proper" triggers everywhere *)
@@ -583,32 +445,8 @@ Section interp_prop.
   (*     specialize (HP R e e eq_refl). destruct HP as (P & _ & _). *)
   (*     rewrite P; eauto. symmetry. assumption. *)
   (*     specialize (HP R e e eq_refl). destruct HP as (P & _ & _). *)
-  (*     rewrite P; eauto.  *)
+  (*     rewrite P; eauto. *)
   (* Qed. *)
-
-  (* Figure 7: Structural law for tau *)
-  Lemma interp_prop_tau :
-    forall E F
-      (h_spec : E ~> PropT F)
-      (k_spec : forall T R, E T -> itree F T -> (T -> itree E R) -> (T -> itree F R) -> itree F R -> Prop)
-      R RR
-      (t_spec : itree E R)
-      (KP : forall T R e t k1 k2, Proper (eutt eq ==> flip impl) (k_spec T R e t k1 k2)),
-      Eq1_PropT _ (interp_prop h_spec k_spec R RR t_spec) (interp_prop h_spec k_spec R RR (Tau t_spec)).
-  Proof.
-    intros.
-    split; [| split].
-    - intros; split; intros.
-      + rewrite <- H.
-        pstep. red. econstructor.
-    (*     left. *)
-    (*     apply H0. *)
-    (*   + rewrite H. *)
-    (*     pinversion H0. subst. *)
-    (*     apply HS. *)
-    (* - red. typeclasses eauto. *)
-        (* - red. typeclasses eauto. *)
-  Admitted.
 
   Lemma interp_prop_ret_inv :
     forall E F
@@ -620,11 +458,7 @@ Section interp_prop.
       (H : interp_prop h_spec k_spec R RR (ret r1) t),
        exists  r2, RR r1 r2 /\ t ≈ ret r2.
   Proof.
-    intros.
-    punfold H.
-    red in H. inversion H; subst.
-    exists r2; eauto.
-  Admitted.
+  Abort.
 
   Lemma interp_prop_vis_inv :
     forall E F
@@ -641,28 +475,6 @@ Section interp_prop.
     intros.
     punfold H.
     red in H. inversion H; subst.
-    apply inj_pair2 in H2.
-    apply inj_pair2 in H3.
-    subst.
-    exists ta. exists k2. auto.
-  Qed.
-
-  Lemma interp_prop_tau_inv :
-    forall E F
-      (h_spec : E ~> PropT F)
-      (k_spec : forall T R, E T -> itree F T -> (T -> itree E R) -> (T -> itree F R) -> itree F R -> Prop)
-      R RR 
-      (s : itree E R)
-      (t : itree F R)
-      (H : interp_prop h_spec k_spec R RR (Tau s) t), 
-      interp_prop h_spec k_spec R RR s t.
-  Proof.
-    intros.
-    punfold H.
-    red in H. inversion H; subst.
-    pclearbot.
-    (* apply HS. *)
-  Admitted.
-  (* Qed. *)
+  Abort.
 
 End interp_prop.
