src/coq/Semantics/InfiniteToFinite.v
@@ -192,7 +192,6 @@ Module EventConvert (LP1 : LLVMParams) (LP2 : LLVMParams) (AC : AddrConvert LP1.
   Require Import String.
 
   Definition L4_convert : Handler E1.L4 E2.L4.
-  Proof.
     refine (fun A e => _).
 
     refine (match e with
@@ -231,7 +230,6 @@ Module EventConvert (LP1 : LLVMParams) (LP2 : LLVMParams) (AC : AddrConvert LP1.
   Defined.
 
   Definition L5_convert : Handler E1.L5 E2.L5.
-  Proof.
     refine (fun A e => _).
 
     refine (match e with
@@ -264,7 +262,6 @@ Module EventConvert (LP1 : LLVMParams) (LP2 : LLVMParams) (AC : AddrConvert LP1.
   Defined.
 
   Definition L6_convert : Handler E1.L6 E2.L6.
-  Proof.
     refine (fun A e => _).
 
     refine (match e with
@@ -373,36 +370,99 @@ Module InfiniteToFinite : LangRefine InterpreterStackBigIntptr InterpreterStack6
   Instance refine_OOM_h_eq_itree {E F T RR} : Proper (eq_itree eq ==> eq_itree eq ==> iff) (@refine_OOM_h E F T RR).
   Admitted.
 
+  From ITree Require Import Eq.EqAxiom.
+
+  Lemma interp_prop_bind :
+    forall R E F
+      (h_spec : E ~> PropT F)
+      (k_spec : forall T R, E T -> itree F T -> (T -> itree E R) -> (T -> itree F R) -> itree F R -> Prop)
+      R' (t : itree E R') (k : R' -> itree E R)
+    , Eq1_PropT _ (interp_prop h_spec k_spec R eq (bind t k))
+                (bind (interp_prop h_spec (fun _ _ _ _ _ _ _ => True) R' eq t)
+                      (fun x => interp_prop h_spec k_spec R eq (k x))).
+  Proof.
+  Admitted.
+
+  (* Lemma interp_propTF_bind : *)
+  (*   forall E F (h_spec : forall T : Type, E T -> PropT F T) k_spec R (RR : relation R) sim *)
+  (*     X (t : itree E X) (k : X -> itree E R) t2, *)
+  (*     interp_PropTF h_spec k_spec RR sim t t-> *)
+  (*     interp_PropTF h_spec k_spec RR sim -> *)
+  (*     interp_PropTF h_spec k_spec RR sim (observe (ITree.bind t k)) t2. *)
+    
+  (* OOM_h (@OOM_spec) (flip RR) (upaco2 (interp_PropT_ E2 E2 OOM_h (@OOM_spec) T (flip RR)) r) *)
+  (*   (observe (ITree.bind (EC.L4_convert A e) (fun x : A => Tau (interp EC.L4_convert (k1 x))))) *)
+  (*   (interp EC.L4_convert t2) *)
+
+  Lemma bind_tau_k:
+    forall {E : Type -> Type} {R : Type} (U : Type) (t : itree E U) (k : U -> itree E R),
+      ITree.bind t (fun x => Tau (k x)) ≅ Tau (ITree.bind t k).
+  Proof.
+    intros.
+    rewrite (itree_eta t).
+    genobs t ot. clear t Heqot. revert ot k.
+    ginit. gcofix CIH; intros.
+    induction ot.
+    - setoid_rewrite bind_ret_l. gstep.
+      reflexivity.
+    - rewrite bind_tau. gstep. constructor.
+      rewrite bind_tau. rewrite (itree_eta t).
+      gfinal. left. eapply CIH.
+    - rewrite 2 bind_vis. gstep.
+  Admitted.
+
   Lemma refine_OOM_h_L4_convert_tree :
     forall T x_inf y_inf RR,
       refine_OOM_h RR x_inf y_inf ->
       refine_OOM_h RR (@L4_convert_tree T x_inf) (@L4_convert_tree T y_inf).
   Proof.
-    (*
     intros T x y RR.
-    unfold L4_convert_tree.
-    unfold InterpreterStackBigIntptr.LP.Events.L4 in *.
+    unfold L4_convert_tree; cbn.
     rewrite (unfold_interp y).
-    revert x y.
+    match goal with
+    | |- context [refine_OOM_h RR (interp EC.L4_convert x) ?r] => remember r
+    end.
+    assert (Heq: i ≅ _interp EC.L4_convert (observe y)). {
+      subst; reflexivity. }
+    clear Heqi.
+    revert x y i Heq.
     pcofix R.
-    intros t u REF.
+    intros t u i Heq REF.
     punfold REF.
     pfold.
     red.
     red in REF.
-    induction REF.
-    - cbn.
-      apply Interp_PropT_Ret with r2.
+    induction REF;
+      apply bisimulation_is_eq in Heq; rewrite Heq; clear Heq; cbn.
+    - apply Interp_PropT_Ret with r2.
       auto.
       rewrite eq2, interp_ret.
       reflexivity.
-    - cbn.
-
-
-    unfold L4_convert_tree in *.
-
-    unfold refine_OOM_h in *.
-     *)
+    - destruct HS; [ | inv H].
+      constructor. right.
+      eapply R; eauto.
+      rewrite unfold_interp. reflexivity.
+    - repeat red in KS, HTA; repeat red in HTA.
+      Opaque EC.L4_convert. destruct e.
+      + eapply interp_PropTF_Proper.
+        intros.
+        admit. admit.
+        rewrite KS.
+        red in HTA. rewrite HTA. unfold trigger.
+        cbn. rewrite interp_bind. rewrite interp_vis, bind_bind.
+        setoid_rewrite interp_ret; setoid_rewrite bind_tau;
+          setoid_rewrite bind_ret_l.
+        reflexivity.
+        unfold subevent, resum, ReSum_inl, cat, resum,
+          Cat_IFun, ReSum_id, inl_, Inl_sum1, id_, Id_IFun.
+        assert (forall (E : Type -> Type) (h_spec : forall T : Type, E T -> PropT E T)
+                  (k_spec : forall T R : Type, E T -> itree E T -> (T -> itree E R) -> (T -> itree E R) -> itree E R -> Prop)
+                  (R : Type) (RR : relation R) (sim : itree E R -> itree E R -> Prop)
+                  X (t : itree E X) k1 k2,
+                   (forall a, Returns a t ->  sim (k1 a) (k2 a)) ->
+                   interp_PropTF h_spec k_spec RR sim (observe (ITree.bind t k1)) (ITree.bind t k2)). admit.
+        eapply H; intros. red in HTA. rewrite HTA in HK.
+        left. pstep. constructor.
   Admitted.
 
   Lemma refine_OOM_h_bind :
